something is wrong with the specification monad

iodiv/DivFreeTauDM.Test.fst
@@ -13,25 +13,61 @@ open IIOSigSpec
 open DivFree.Test
 open DivFreeTauSpec.Test
 
-let th #a = theta #a #io_sig iodiv_act
+open TauIODiv
 
+let lift_i (w:iwp 'a) (#index:Type0) : index -> iwp (either index unit) =
+  (fun i -> i_bind_alt w (fun _ -> i_ret (Inl i)))
 
-let test1 (fd:file_descr) : Lemma (th (body1 fd) `ile` ibody1 fd) = ()
+let iodiv_repeat #a #w (f :  iodiv_dm a w) : iodiv_dm unit (i_iter (lift_i w) ()) =
+  let f' : i:unit -> iodiv_dm (either unit unit) (lift_i w i) =
+    fun i -> iodiv_bind _ _ _ _ f (fun _ -> iodiv_ret _ (Inl i)) in
+  iodiv_iter f' ()
 
-#set-options "--split_queries always"
-let test2 (fd:file_descr) =
-  let body' = lift_body (ibody1 fd) in
-//  pre1_inv1 fd;
-//  let body_inv = repeat_body_inv #unit (fun _ -> pre1 fd) (inv1 fd) in
+let lem_spec_to_loop
+  (a:Type)
+  (pre0 : trace -> Type0)
+  (inv0 : trace -> Type0)
+  (pre0_inv0 : squash (forall h lt. pre0 h /\ inv0 lt ==> pre0 (rev_acc lt h))) :
+  Lemma (
+    let body0 : iwp a = iprepost pre0 (fun h r -> terminates r /\ inv0 (_trace r)) in
+    let loop0 : iwp unit = iprepost pre0 (fun h r -> diverges r /\ repeat_inv_post inv0 r) in
+    i_iter (lift_i body0) () `ile` loop0) =
+  let body0 : iwp a = iprepost pre0 (fun h r -> terminates r /\ inv0 (_trace r)) in
+  let loop0 = iprepost pre0 (fun h r -> diverges r /\ repeat_inv_post inv0 r) in
+  let body' = lift_i body0 in
+  let body_inv = repeat_body_inv #unit (fun _ -> pre0) inv0 in
+  assert (body' () `ile` body_inv ());
+  i_iter_mono #unit body' body_inv ();
+  assert ((i_iter body' ()) `ile` (i_iter body_inv ()));
+  repeat_inv_proof (fun _ -> pre0) inv0 () ;
+  assert (i_iter body_inv () `ile` repeat_inv (fun _ -> pre0) inv0 ());
+  assert (repeat_inv (fun _ -> pre0) inv0 () `ile` loop0);
+  assert (i_iter body' () `ile` loop0)
 
-  test1 fd;
+let lem_body_to_loop
+  (#a:Type)
+  (#pre0 : trace -> Type0)
+  (#inv0 : trace -> Type0)
+  (#pre0_inv0 : squash (forall h lt. pre0 h /\ inv0 lt ==> pre0 (rev_acc lt h))) 
+  (f : iodiv_dm a (iprepost pre0 (fun h r -> terminates r /\ inv0 (_trace r)))) :
+  Lemma (
+    let body0 : iwp a = iprepost pre0 (fun h r -> terminates r /\ inv0 (_trace r)) in
+    let loop0 : iwp unit = iprepost pre0 (fun h r -> diverges r /\ repeat_inv_post inv0 r) in
+    i_iter (lift_i body0) () `ile` loop0) =
+  lem_spec_to_loop a pre0 inv0 pre0_inv0
 
-  assert (th (m_bind (body1 fd) (fun msg -> m_ret (Inl ()))) `ile` i_bind #_ #(either unit string) (ibody1 fd) (fun _ -> i_ret (Inl ())));
-  assert (th (m_bind (body1 fd) (fun msg -> m_ret (Inl ()))) `ile` lift_body (ibody1 fd) ());
-  //repeat_inv_proof #unit (fun _ -> (pre1 fd)) (inv1 fd) () ;
-  //i_iter_mono (fun _ -> repeat_body_inv (fun _ -> (pre1 fd)) (inv1 fd) ()) (repeat_body_inv (fun _ -> (pre1 fd)) (inv1 fd)) () ;
-  assume (th (m_iter (fun i -> m_bind (body1 fd) (fun msg -> m_ret (Inl i))) ()) `ile` i_iter (lift_body (ibody1 fd)) ());
-  assert (th (m_iter (body1' fd) ()) `ile` i_iter body' ());
-  assert (th (loop1 fd) `ile` i_iter body' ());
-  itest1 fd;
-  assert (th (loop1 fd) `ile` iloop1 fd)
+let dm_body1 (fd:file_descr) : iodiv_dm string (ibody1 fd) = body1 fd
+
+let dm_loop1 (fd:file_descr) : iodiv_dm unit (iloop1 fd) = 
+  lem_body_to_loop (dm_body1 fd);
+  iodiv_repeat (dm_body1 fd)
+
+(** ** Test print 0 1 **)
+
+let dm_body2 : iodiv_dm unit (iprepost (fun _ -> True) (fun h r -> terminates r /\ _trace r == [EPrint "0";EPrint "1"])) = 
+  (m_bind (m_call Print "0") (fun () -> m_call Print "1"))
+
+let iloop2 : iwp unit = iprepost (fun _ -> True) (fun h r -> diverges r /\ False) //repeat_inv_post (fun lt -> lt == [EPrint "0"; EPrint "3:"]) r)
+
+let dm_loop2 () : iodiv_dm unit iloop2  =
+  iodiv_repeat dm_body2
